thermostat.v
@@ -1,0 +1,355 @@
+Require Import List.
+Require Import util.
+Require Import list_util.
+Require Import c_geometry.
+Require Import c_monotonic_flow.
+Require c_concrete.
+Require c_abstract.
+Require c_abstraction.
+Require c_square_abstraction.
+Require abstract_as_graph.
+Require Import CRln.
+Require Import CRexp.
+Set Implicit Arguments.
+
+Open Local Scope CR_scope.
+
+Definition centi: Q := (1#100).
+
+Definition r01: Range. exists ('0, '1); CRle_constants. Defined.
+Definition r15_1: Range. exists ('(1#2), '1); CRle_constants. Defined.
+Definition r1_2: Range. exists ('1, '2); CRle_constants. Defined.
+Definition r2_3: Range. exists ('2, '3); CRle_constants. Defined.
+Definition r45_5: Range. exists ('(9#2), '5); CRle_constants. Defined.
+Definition r5_6: Range. exists ('5, '6); CRle_constants. Defined.
+Definition r6_9: Range. exists ('6, '9); CRle_constants. Defined.
+Definition r9_10: Range. exists ('9, '10); CRle_constants. Defined.
+Definition r5_10: Range. exists ('5, '10); CRle_constants. Defined.
+Definition rC_10: Range. exists ('centi, '10); CRle_constants. Defined.
+
+Inductive Location: Set := Heat | Cool | Check.
+
+Definition Location_eq_dec (l l': Location): decision (l=l'). dec_eq. Defined.
+
+Definition locations: list Location := Heat :: Cool :: Check :: nil.
+
+Lemma NoDup_locations: NoDup locations.
+  apply decision_true with (NoDup_dec Location_eq_dec locations).
+  vm_compute. reflexivity.
+Qed.
+
+Lemma locations_complete l: In l locations.
+Proof. destruct l; compute; tauto. Qed.
+
+Let State : Type := (Location * Point)%type.
+
+Definition point: State -> Point := snd.
+Definition loc: State -> Location := fst.
+Definition clock: State -> CR := fst ∘ point.
+Definition temp: State -> CR := snd ∘ point.
+
+Definition world: OpenSquare := unbounded_square.
+
+Definition above (c: CR): OpenRange := existT OCRle (Some c, None) I.
+Definition below (c: CR): OpenRange := existT OCRle (None, Some c) I.
+
+
+Definition invariant (s: State): Prop :=
+  'centi <= temp s /\
+  match loc s with
+  | Heat => temp s <= '10 /\ clock s <= '3
+  | Cool => '5 <= temp s
+  | Check => clock s <= '1
+  end.
+
+Let PointCSetoid: CSetoid := ProdCSetoid CRasCSetoid CRasCSetoid.
+
+Lemma invariant_wd: forall l l', l = l' ->
+  forall (p p': PointCSetoid), p[=]p' -> (invariant (l, p) <-> invariant (l', p')).
+Proof with auto.
+  unfold invariant.
+  intros l l' le. subst.
+  intros [x y] [x' y'] pe.
+  inversion_clear pe.
+  simpl loc. unfold temp, clock. unfold compose. simpl @fst. simpl @snd.
+  destruct l'; try rewrite H; try rewrite H0; split...
+Qed.
+
+Definition invariant_squares (l: Location): OpenSquare :=
+  match l with
+  | Cool => (unbounded_range, above ('5))
+  | Heat => (below ('3), rC_10: OpenRange)
+  | Check => (below ('1), above ('centi))
+  end.
+
+Lemma invariant_squares_correct (l : Location) (p : Point):
+  invariant (l, p) -> in_osquare p (invariant_squares l).
+Proof.
+  unfold invariant, in_osquare, in_orange, orange_left, orange_right.
+  destruct l; simpl; intuition.
+Qed.
+
+Definition initial_square: OpenSquare := (r01: OpenRange, r5_10: OpenRange).
+Definition initial_location := Heat.
+Definition initial (s: State): Prop :=
+  loc s = initial_location /\ in_osquare (point s) initial_square.
+
+Lemma initial_invariant (s: State): initial s -> invariant s.
+Proof with auto.
+  destruct s as [l [c t]].
+  unfold initial, invariant, initial_square.
+  simpl.
+  intros [H [[H0 H1] [H2 H3]]].
+  subst.
+  unfold initial_location, temp, clock, compose.
+  simpl in *.
+  split...
+    apply CRle_trans with ('5)...
+    CRle_constants.
+  split...
+  apply CRle_trans with ('1)...
+  CRle_constants.
+Qed.
+
+Definition clock_flow (l: Location): Flow CRasCSetoid := c_flow.positive_linear.f 1.
+
+Definition temp_flow (l: Location): Flow CRasCSetoid :=
+  match l with
+  | Heat => c_flow.positive_linear.f 2
+  | Cool => c_flow.decreasing_exponential.f
+  | Check => c_flow.scale.flow ('(1#2)) c_flow.decreasing_exponential.f
+  end.
+
+Definition clock_flow_inv (l: Location) (a b: OpenRange): OpenRange :=
+  c_square_flow_conditions.one_axis.flow_range
+    _ (c_flow.positive_linear.inv_correct 1) (c_flow.positive_linear.mono 1) a b.
+
+Lemma half_pos: '0 < '(1#2).
+Proof. apply CRlt_Qlt. reflexivity. Qed.
+
+Definition temp_flow_inv (l: Location) (a b: OpenRange): OpenRange :=
+  match l with
+  | Heat => c_square_flow_conditions.one_axis.flow_range
+    _ (c_flow.positive_linear.inv_correct 2) (c_flow.positive_linear.mono 2) a b
+  | Cool => c_flow.decreasing_exponential.inv a b
+  | Check => c_flow.scale.inv half_pos c_flow.decreasing_exponential.inv a b
+  end.
+
+Lemma clock_rfis l: range_flow_inv_spec (clock_flow l) (clock_flow_inv l).
+Proof with auto.
+  intro.
+  unfold range_flow_inv_spec. intros.
+  apply c_square_flow_conditions.one_axis.flow_range_covers with p...
+Qed.
+
+Lemma temp_rfis l: range_flow_inv_spec (temp_flow l) (temp_flow_inv l).
+Proof with auto.
+  destruct l; simpl temp_flow.
+      unfold range_flow_inv_spec. intros.
+      apply c_square_flow_conditions.one_axis.flow_range_covers with p...
+    apply c_flow.decreasing_exponential.inv_correct.
+  apply c_flow.scale.inv_correct, c_flow.decreasing_exponential.inv_correct.
+Qed.
+
+Definition clock_reset (l l': Location) (c: CR): CR :=
+  match l, l' with
+  | Cool, Heat => '0
+  | Heat, Check => '0
+  | Check, Heat => '0
+  | _, _ => c (* dummy *)
+  end.
+
+Definition temp_reset (l l': Location) (t: CR): CR := t. (* cannot reset temperature *)
+
+Definition reset (l l': Location) (p: Point): Point :=
+  (clock_reset l l' (fst p), temp_reset l l' (snd p)).
+
+Lemma clock_reset_inc l l': increasing (clock_reset l l').
+Proof with auto.
+  do 5 intro.
+  unfold clock_reset.
+  destruct l; destruct l'...
+Qed.
+
+Lemma temp_reset_inc l l': increasing (temp_reset l l').
+Proof. intros. intro. auto. Qed.
+
+Definition guard_square (l l': Location): option OpenSquare :=
+  match l, l' with
+  | Heat, Cool => Some (unbounded_range, above ('9))
+  | Cool, Heat => Some (unbounded_range, below ('6))
+  | Heat, Check => Some (above ('2), unbounded_range)
+  | Check, Heat => Some (above ('(1#2)), unbounded_range)
+  | _, _ => None
+  end.
+
+Definition guard (s: State) (l: Location): Prop :=
+  match guard_square (fst s) l with
+  | None => False
+  | Some q => in_osquare (snd s) q
+  end.
+
+Definition concrete_system: c_concrete.System :=
+  @c_concrete.Build_System PointCSetoid Location Location_eq_dec
+  locations locations_complete NoDup_locations initial invariant
+  initial_invariant invariant_wd
+  (fun l => product_flow (clock_flow l) (temp_flow l)) guard reset.
+
+(* intervals: *)
+
+Inductive ClockInterval: Set := CI_15 | CI15_1 | CI1_2 | CI2_3 | CI3_.
+Inductive TempInterval: Set := TI_45 | TI45_5 | TI5_6 | TI6_9 | TI9_10 | TI10_.
+
+Definition ClockInterval_eq_dec (i i': ClockInterval): decision (i=i'). dec_eq. Defined.
+Definition TempInterval_eq_dec (i i': TempInterval): decision (i=i'). dec_eq. Defined.
+
+Definition ClockInterval_bounds (i: ClockInterval): OpenRange :=
+  match i with
+  | CI_15 => below ('(1#2))
+  | CI15_1 => r15_1 | CI1_2 => r1_2 | CI2_3 => r2_3
+  | CI3_ => above ('3)
+  end.
+
+Definition TempInterval_bounds (i: TempInterval): OpenRange :=
+  match i with
+  | TI_45 => below ('(9#2))
+  | TI45_5 => r45_5
+  | TI5_6 => r5_6
+  | TI6_9 => r6_9
+  | TI9_10 => r9_10
+  | TI10_ => above ('10)
+  end.
+
+Definition clock_intervals: list ClockInterval := CI_15 :: CI15_1 :: CI1_2 :: CI2_3 :: CI3_ :: nil.
+Definition temp_intervals: list TempInterval := TI_45 :: TI45_5 :: TI5_6 :: TI6_9 :: TI9_10 :: TI10_ :: nil.
+
+Lemma clock_intervals_complete: forall i, List.In i clock_intervals.
+Proof. destruct i; compute; tauto. Qed.
+
+Lemma temp_intervals_complete: forall i, List.In i temp_intervals.
+Proof. destruct i; compute; tauto. Qed.
+
+Lemma NoDup_clock_intervals: NoDup clock_intervals.
+  apply decision_true with (NoDup_dec ClockInterval_eq_dec clock_intervals).
+  vm_compute. ref.
+Qed.
+
+Lemma NoDup_temp_intervals: NoDup temp_intervals.
+  apply decision_true with (NoDup_dec TempInterval_eq_dec temp_intervals).
+  vm_compute. ref.
+Qed.
+
+Definition s_absClockInterval (r: CR):
+  { i: ClockInterval | in_orange (ClockInterval_bounds i) r }.
+Proof with auto.
+  intro.
+  unfold in_orange, orange_left, orange_right.
+  destruct (CR_le_le_dec r ('(1#2))). exists CI_15. simpl...
+  destruct (CR_le_le_dec r ('1)). exists CI15_1...
+  destruct (CR_le_le_dec r ('2)). exists CI1_2...
+  destruct (CR_le_le_dec r ('3)). exists CI2_3...
+  exists CI3_. simpl...
+Defined.
+
+Definition s_absTempInterval (r: CR):
+  { i: TempInterval | in_orange (TempInterval_bounds i) r }.
+Proof with auto.
+  intro.
+  unfold in_orange, orange_left, orange_right.
+  destruct (CR_le_le_dec r ('(9#2))). exists TI_45. simpl...
+  destruct (CR_le_le_dec r ('5)). exists TI45_5...
+  destruct (CR_le_le_dec r ('6)). exists TI5_6...
+  destruct (CR_le_le_dec r ('9)). exists TI6_9...
+  destruct (CR_le_le_dec r ('10)). exists TI9_10...
+  exists TI10_. simpl...
+Defined.
+
+Definition absClockInterval (r: CR): ClockInterval := proj1_sig (s_absClockInterval r).
+Definition absTempInterval (r: CR): TempInterval := proj1_sig (s_absTempInterval r).
+
+Lemma regions_cover_invariants l (p: c_concrete.Point concrete_system):
+  c_concrete.invariant (l, p) ->
+  c_square_abstraction.in_region ClockInterval_bounds TempInterval_bounds p
+    (c_square_abstraction.absInterval absClockInterval absTempInterval p).
+Proof with auto.
+  simpl c_concrete.invariant.
+  destruct p.
+  intros.
+  unfold c_square_abstraction.in_region.
+  unfold c_square_abstraction.absInterval.
+  simpl.
+  unfold absClockInterval, absTempInterval.
+  destruct (s_absClockInterval c). destruct (s_absTempInterval c0). simpl.
+  split...
+Qed.
+
+Let Region := c_square_abstraction.SquareInterval ClockInterval TempInterval.
+
+Definition guard_dec eps (ls : Location * Region * Location) :=
+  let (lr, l2) := ls in
+  let (l1, r) := lr in
+    match guard_square l1 l2 with
+    | Some s => osquares_overlap_dec eps (s,
+        c_square_abstraction.square ClockInterval_bounds TempInterval_bounds r)
+    | None => false
+    end.
+
+Lemma over_guard eps : 
+  guard_dec eps >=> c_square_abstraction.abstract_guard ClockInterval_bounds TempInterval_bounds guard.
+Proof with auto.
+  intros eps [[l r] l'] gf [p [in_p g]].
+  unfold guard_dec in gf. unfold guard in g.
+  simpl @fst in *. simpl @snd in *.  
+  destruct (guard_square l l'); try contradiction.
+  apply (over_osquares_overlap eps gf).
+  apply osquares_share_point with p...
+Qed.
+
+Definition initial_dec eps :=
+  c_square_abstraction.initial_dec (Location:=Location) 
+    Location_eq_dec ClockInterval_bounds TempInterval_bounds initial_location initial_square eps.
+
+Lemma over_initial eps : 
+  initial_dec eps >=> 
+  c_abstraction.initial_condition concrete_system 
+  (c_square_abstraction.in_region ClockInterval_bounds TempInterval_bounds).
+Proof with auto.
+  apply c_square_abstraction.over_initial.
+  intros. destruct s...
+Qed.
+
+Definition abstract_system (eps : Qpos) : c_abstract.System concrete_system.
+Proof with auto.
+  intro eps. eapply c_abstraction.abstract_system.
+              eexact (c_square_abstraction.SquareInterval_eq_dec ClockInterval_eq_dec TempInterval_eq_dec).
+            eexact (c_square_abstraction.squareIntervals_complete _ clock_intervals_complete _ temp_intervals_complete).
+          eexact (c_square_abstraction.NoDup_squareIntervals NoDup_clock_intervals NoDup_temp_intervals).
+        eapply (@c_square_abstraction.do_cont_trans Location ClockInterval TempInterval Location_eq_dec locations locations_complete ClockInterval_bounds TempInterval_bounds clock_flow temp_flow clock_flow_inv temp_flow_inv).
+              apply clock_rfis.
+            apply temp_rfis.
+          eexact invariant_squares_correct.
+        exact eps.
+      eapply c_square_abstraction.do_odisc_trans.
+                eexact invariant_squares_correct.
+              eexact clock_reset_inc.
+            eexact temp_reset_inc.
+          destruct p; ref.
+        eexact (mk_DO (over_guard eps)).
+      eexact eps.
+    eexact (mk_DO (over_initial eps)).
+  unfold c_abstraction.RegionsCoverInvariants.
+  eexact regions_cover_invariants.
+Defined.
+
+Print Assumptions abstract_system.
+
+Definition abs_sys: c_abstract.System concrete_system := abstract_system (1#100).
+
+Definition vs := abstract_as_graph.vertices abs_sys.
+Definition g := abstract_as_graph.g abs_sys.
+Definition graph := flat_map (@digraph.edges g) vs.
+
+(* Eval vm_compute in vs. *)
+Eval vm_compute in (List.length graph).
+  (* causes an assertion failure in this version of Coq.. *)
+
